Begin rewrite

coq/Core.v
@@ -5,321 +5,8 @@ Unset Strict Implicit.
 Unset Printing Implicit Defensive.
 Set Bullet Behavior "Strict Subproofs".
 
-Require Vector.
+Load Exp.
 
-Definition polynomial := seq (Set * nat).
-Print nth.
-
-Definition zterm : Set * nat := (Empty_set , 0).
-
-
-Unset Elimination Schemes.
-Inductive poly_fix (p : polynomial) : Type :=
-  | var : nat -> poly_fix p
-  | con : forall n, fst (nth zterm p n) ->
-                     Vector.t (poly_fix p) (snd (nth zterm p n)) ->
-                     poly_fix p.
-Set Elimination Schemes.
-
-Arguments var {p}.
-Arguments con {p}.
-
-(*Stronger induction principle w/ better subterm knowledge *)
-Fixpoint poly_fix_ind {p}
-         (P : poly_fix p -> Prop)
-         (IHV : forall n, P(var n))
-         (IHC : forall n s v,
-             Vector.fold_right (fun t : poly_fix p => and (P t)) v True ->
-             P (con n s v))
-         (e : poly_fix p) { struct e} : P e :=
-  match e with
-  | var n => IHV n
-  | con n s v =>
-    let fix loop n v :=
-        match v return Vector.fold_right (fun t => and (P t)) v True with
-        | Vector.nil => I
-        | Vector.cons e' n v' => conj (poly_fix_ind IHV IHC e') (loop n v')
-        end in
-    IHC n s v (loop _ v)
-  end.
-
-Notation "[*]" := (Vector.nil _).
-Notation "[* x ]" := (Vector.cons _ _ x (Vector.nil _)).
-Notation "[* x ; .. ; y ]" := (Vector.cons _ x _ .. (Vector.cons _ y _ (Vector.nil _)) ..).
-
-Notation "[ n | s , v ]" := (con n s v).
-Notation "[{ p } n | s , v ]" := (@con p n s v).
-
-
-Definition test1 : polynomial := [:: (unit,1) ; (unit,2) ; (nat,0)].
-
-Definition tvar (n : nat) : poly_fix test1 :=
-  [{test1} 2 | n, [*]].
-
-Definition prod_test : Vector.t nat 1 := [* 3].
-Definition prod_test2 : Vector.t nat 3 := [* 3; 5; 4].
-
-Definition tlam (e : poly_fix test1) : poly_fix test1 :=
-  [{test1} 0 | tt , [* e]].
-
-Definition tapp (e1 e2 : poly_fix test1) : poly_fix test1 :=
-  [{test1} 1 | tt, [* e1; e2]].
-
-
-Definition test1ex : poly_fix test1 := tlam (tlam (tapp (tvar 1) (tvar 0))).
-
-Inductive ctxt_var p : Type :=
-| term_var : poly_fix p -> ctxt_var p
-| sort_var : ctxt_var p.
-
-Arguments term_var {p} e.
-Arguments sort_var {p}.
-
-Definition ctxt p := list (ctxt_var p).
-
-(* terms form a category over sorts w/ (empty or constant?) Γ *)
-(* Well-typed sorts are those which are related to themselves by the sort rules of a language*)
-Definition sort_rule p : Type := (ctxt p * ctxt p) * (poly_fix p * poly_fix p).
-
-(* Well-typed terms are those which are related to themselves by the sort rules of a language*)
-Definition term_rule p : Type :=
-  (ctxt p * ctxt p) * (poly_fix p * poly_fix p) * (poly_fix p * poly_fix p).
-
-(* TODO: inline these or no? *)
-Inductive rule (p : polynomial) : Type :=
-| sort : ctxt p -> ctxt p -> poly_fix p -> poly_fix p -> rule p
-| term : ctxt p -> ctxt p -> poly_fix p -> poly_fix p -> poly_fix p -> poly_fix p ->  rule p.
-
-Bind Scope rule_scope with rule.
-Delimit Scope rule_scope with rule.
-Local Open Scope rule_scope.
-Notation "{r c1 <# c2 |- s1 <# s2 }" := (sort c1 c2 s1 s2) (at level 80) : rule_scope.
-Notation "{r c |- s1 <# s2 }" := (sort c c s1 s2) (at level 80):rule_scope.
-Notation "{r c |- s }" := (sort c c s s) (at level 80):rule_scope.
-Notation "{r c1 <# c2 |- e1 <# e2 .: s1 <# s2 }" :=
-  (term c1 c2 e1 e2 s1 s2) (at level 80) : rule_scope.
-Notation "{r c |- e1 <# e2 .: s1 <# s2 }" :=
-  (term c c e1 e2 s1 s2) (at level 80) : rule_scope.
-Notation "{r c |- e1 <# e2 .: s }" :=
-  ({r c |- e1 <# e2 .: s <# s}) (at level 80) : rule_scope.
-Notation "{r c |- e .: s }" := 
-  ({r c |- e <# e.: s}) (at level 80) : rule_scope.
-
-Definition lang p := list (rule p).
-
-(*EXAMPLE*)
-(* syntax of single explicit substitutions *)
-Definition subst_syn : polynomial :=
-  [:: (nat, 0); (* var (deBruijn) *)
-     (unit, 2) (*subst M[N/0] *)
-  ].
-
-Definition sub (m n : poly_fix subst_syn) : poly_fix subst_syn :=
-  [{subst_syn} 1 | tt , [* m; n]].
-
-Definition svar (n : nat) : poly_fix subst_syn :=
-  [{subst_syn} 0 | n , [*]].
-
-  (* equational theory of substitutions *)
-Definition subst_lang : lang subst_syn :=
-  [:: {r [:: sort_var] |- sub (svar 0) (var 0) <# var 0};
-     {r[:: sort_var; sort_var] |- [{subst_syn} 1 | tt, [* var 0; var 1]]};
-     {r[:: sort_var; sort_var; term_var (var 1)] |- [{subst_syn} 1 | tt, [* var 0; var 2]]};
-     {r[:: sort_var; term_var (var 0); sort_var] |-
-      [{subst_syn} 1 | tt, [* var 1; var 2]] .: var 0};
-     {r[:: sort_var; term_var (var 0); sort_var; term_var (var 2)] |-
-      [{subst_syn} 1 | tt, [* var 1; var 3]] .: var 0}
-  ].
-
-  (*TODO: finish axioms
-    (wf_sort_and_cong ([:: sort_var _; sort_var _],
-                       Ccon [++ tt | [* Cvar _ 0; Cvar _ 1]]))
-      ++ (wf_sort_and_cong ([:: sort_var _; sort_var _; term_var (Cvar _ 1)],
-                       Ccon [++ tt | [* Cvar _ 0; Cvar _ 2]]))
-      ++ (wf_sort_and_cong ([:: sort_var _; term_var (Cvar _ 0); sort_var _],
-                       Ccon [++ tt | [* Cvar _ 1; Cvar _ 2]]))
-      ++ (wf_sort_and_cong ([:: sort_var _; term_var (Cvar _ 0); sort_var _; term_var (Cvar _ 2)],
-                            Ccon [++ tt | [* Cvar _ 1; Cvar _ 3]])).
-      *)
-
-Definition psubst (p : polynomial) := seq (poly_fix p).
-
-Fixpoint var_lookup {p} (c : psubst p) (n : nat) : poly_fix p :=
-  match c , n with
-  | [::], _ => var n (*keep the var if no substitution needed*)
-  | e :: _, 0 => e (*use the element if one is found *)
-  | _ :: c', n'.+1 => var_lookup c' n' (*otherwise decrease both and continue *)
-  end.
-
-Fixpoint exp_subst {p} (e : poly_fix p) (s : psubst p) : poly_fix p :=
-  match e with
-  | var n => var_lookup s n
-  | con n s' v => con n s' (Vector.map (fun e => exp_subst e s) v)
-  end.
-
-(*TODO: this is in the library. Why can't I find it? *)
-Lemma sub_0_r : forall n, n - 0 = n.
-Proof.
-  elim; done.
-Qed.  
-
-Lemma lookup_ge : forall p c n, length c <= n -> @var_lookup p c n = var (n - size c).
-Proof.
-  move => p; elim.
-  move => n _;
-  rewrite sub_0_r //=.
-  move => x l IH; elim.
-  rewrite ltn0; done.
-  move => n _.
-  apply: IH.
-Qed.
-
-Lemma lookup_nth : forall p c n, @var_lookup p c n = nth (var (n - size c)) c n.
-Proof.
-  move => p; elim.
-  move => n;
-  rewrite sub_0_r nth_nil //=.
-  move => x l IH; elim;[done|].
-  move => n _;
-  apply: IH.
-Qed.  
-
-(*TODO*)
-(* Well-scoped languages
-   a presupposition of well-formed languages
-   Written as functions that decide the properties
- *)
-
-Fixpoint ws_exp {p : polynomial} csz (e : poly_fix p) : bool :=
-  match e with
-  | var n => n < csz
-  | con n s v => Vector.fold_right (fun e f => (ws_exp csz e) && f) v true
-  end.
-
-Definition ws_ctxt_var {p : polynomial} csz (v : ctxt_var p) : bool :=
-  match v with
-  | sort_var => true
-  | term_var ty => ws_exp csz ty
-  end.
-
-Fixpoint ws_ctxt {p : polynomial} (c : ctxt p) : bool :=
-  match c with
-  | [::] => true
-  | v :: c' => ws_ctxt c' && ws_ctxt_var (size c) v
-  end.
-
-Fixpoint ws_lang {p : polynomial} (l : lang p) : bool :=
-  match l with
-  |[::] => true
-  | {r c1 <# c2 |- s1 <# s2} :: l' => ws_lang l' && ws_exp (size c1) s1 && ws_exp (size c2) s2
-  | {r c1 <# c2 |- e1 <# e2 .: s1 <# s2} :: l' =>
-    ws_lang l' && ws_exp (size c1) e1 && ws_exp (size c2) e2
-            && ws_exp (size c1) s1 && ws_exp (size c2) s2
-  end%rule.
-
-(* replaces m variables with terms with n free vars*)
-Definition ws_subst {p} n (s : psubst p) m : bool :=
-  (List.fold_right (fun e b => ws_exp n e && b) true s) && (size s == m).
-
-
-Lemma unandb : forall (a b : bool) (C : Prop), (a -> b -> C) <-> (a && b -> C).
-Proof.
-  move => a b C; split.
-  - move => CF ab.
-    apply andb_prop in ab.
-    case: ab.
-    done.
-  - move => CF aa bb.
-    apply CF.
-    rewrite andb_true_intro //=.
-Qed.
-
-Lemma ws_nth : forall p n (s : psubst p) m e n',
-    ws_subst n s m -> ws_exp n e -> ws_exp n (nth e s n').
-Proof.
-  move => p n ; elim.
-  - move => m e; elim; [done|].
-    move => n' IH //=.
-  - move => x l IH m e.
-    elim => [| n' _].
-    + rewrite /ws_subst //=.
-      repeat case /andb_prop.
-      done.
-    + rewrite /ws_subst //=.
-      repeat case /andb_prop.
-      move => _ lf wse.
-      case: m wse => //= m.
-      rewrite eqSS => wse.
-      apply: IH.
-      rewrite /ws_subst //=.
-      apply andb_true_intro; split. 
-      done.
-      exact wse.
-Qed.
-
-Lemma ws_empty : forall p n m, @ws_subst p n [::] m = (m == 0).
-Proof.
-  move => p n m.
-  rewrite /ws_subst //=.
-Qed.
-
-Lemma ws_lookup : forall p n (s : psubst p) (m n' : nat),
-    ws_subst n s m -> n' < m -> ws_exp n (var_lookup s n').
-Proof.  
-  move => p n.
-  elim.  
-  - move => m;
-    elim;
-    move: ws_empty ->;
-    [ move => /eqP -> //=
-    | move => n' IH //= /eqP => -> //=].
-  - move => e l IH m n'.
-    rewrite /ws_subst => //=.
-    (repeat case /andP) => wse sl sr.
-    elim: n' => [ //= | n' _ n'lt].
-    case: m sr n'lt => //= m.
-    move: eqSS -> => n'lt ngm.
-    apply: (IH m n') => //=.
-    rewrite /ws_subst //=.
-    move: n'lt ->.
-    rewrite Bool.andb_true_r //=.
-Qed.
-
-Ltac ws_simpl :=
-  match goal with
-    (* break up ws_subst *)
-    [ |- is_true (ws_subst _ _ _) -> _] =>
-    rewrite /ws_subst;
-    case /andP
-  end.
-
-
-Theorem subst_preserves_ws
-  : forall {p} e (s : psubst p) (c c' : ctxt p),
-    ws_exp (size c') e ->
-    ws_subst (size c) s (size c') ->
-    ws_exp (size c) (exp_subst e s).
-Proof.
-  move => p e s c c' wse.
-  move => wss.
-  pose (wss' := wss).
-  move: wss'.
-  ws_simpl.
-  move => elem_ws size_eq.
-  pose size_eq' := size_eq.
-  move: size_eq' wse => /eqP <-.
-  elim: e => //= => n.
-  - apply: ws_lookup => //=;
-    move: size_eq => /eqP -> //=.
-  - move => _.
-    elim => //= x n' v IHA IHB.
-    case /andP => xexp rexp.
-    case: IHB => IHB1 IHB2.
-    apply /andP. split; [auto|].
-    move: IHA -> => //=.
-Qed.
-
-(* TODO: from here*)
 (* We could embed well-scopedness in bool, but well-typedness can be undecideable,
    so we leave it in Prop.
    Some constructors take in more presuppositions than strictly necessary
@@ -327,160 +14,378 @@ Qed.
    It is easier to devise secondary "constructor" functions that perform these
    derivations than to do the mutually inductive proof that such derivations exist.
  *)
-(* TODO: build in transitivity? *)
-Inductive wf_sort {p} : lang p -> ctxt p -> ctxt p -> poly_fix p -> poly_fix p -> Prop :=
-| wf_sort_by : forall l c1 c2 t1 t2 s1 s2 c1' c2',
+Inductive wf_sort {p} : lang p -> ctx p -> exp p -> Prop :=
+| wf_sort_by : forall l c t,
     (* presuppositions *)
     wf_lang l ->
-    wf_ctxt l c1 c2 ->
+    wf_ctx l c ->
     (* well-formed input *)
-    wf_sort l c1 c2 t1 t2 ->
-    wf_subst l c1 c2 s1 s2 c1' c2' ->
-    List.In ({r c1' <# c2'|- t1 <# t2}%rule) l ->
-    wf_sort l c1 c2 (exp_subst t1 s1) (exp_subst t2 s2)
-| wf_sort_trans : forall l c1 c2 c3 t1 t2 t3,
+    List.In ({| c|- t}) l ->
+    wf_sort l c t
+| wf_sort_subst : forall l c s c' t',
     (* presuppositions *)
     wf_lang l ->
-    wf_ctxt l c1 c3 ->
+    wf_ctx l c ->
     (* well-formed input *)
-    wf_sort l c1 c2 t1 t2 ->
-    wf_sort l c2 c3 t2 t3 ->
-    wf_sort l c1 c3 t1 t3
-with wf_term {p} : lang p ->
-                   ctxt p -> ctxt p ->
-                   poly_fix p -> poly_fix p ->
-                   poly_fix p -> poly_fix p -> Prop :=
-| wf_term_by : forall l c1 c2 e1 e2 t1 t2 s1 s2 c1' c2',
+    wf_subst l c s c' ->
+    wf_sort l c' t' ->
+    wf_sort l c t'[/s/]
+with le_sort {p} : lang p -> ctx p -> ctx p -> exp p -> exp p -> Prop :=
+| le_sort_by : forall l c1 c2 t1 t2,
     (* presuppositions *)
     wf_lang l ->
-    wf_ctxt l c1 c2 ->
-    wf_sort l c1 c2 (exp_subst t1 s1) (exp_subst t2 s2) ->
+    wf_ctx l c1 ->
+    wf_ctx l c2 ->
+    le_ctx l c1 c2 ->
+    wf_sort l c1 t1 ->
+    wf_sort l c1 t2 ->
     (* well-formed input *)
-    wf_subst l c1 c2 s1 s2 c1' c2' ->
-    List.In ({r c1' <# c2' |- e1 <# e2.: t1 <# t2}%rule) l ->
-    wf_term l c1 c2 (exp_subst e1 s1) (exp_subst e2 s2) (exp_subst t1 s1) (exp_subst t2 s2)
-| wf_term_trans : forall l c1 c2 c3 e1 e2 e3 t1 t2 t3,
+    List.In ({< c1 <# c2 |- t1 <# t2}) l ->
+    le_sort l c1 c2 t1 t2
+| le_sort_subst : forall l c1 c2 s1 s2 c1' c2' t1' t2',
     (* presuppositions *)
     wf_lang l ->
-    wf_ctxt l c1 c3 ->
-    wf_sort l c1 c3 t1 t3 ->
+    wf_ctx l c1 ->
+    wf_ctx l c2 ->
+    le_ctx l c1 c2 ->
+    wf_sort l c1 t1'[/s1/] ->
+    wf_sort l c1 t2'[/s2/] ->
     (* well-formed input *)
-    wf_term l c1 c2 e1 e2 t1 t2 ->
-    wf_term l c2 c3 e2 e3 t2 t3 ->
-    wf_term l c1 c3 e1 e3 t1 t3
-(* TODO: these rules are experimental; check *)
-| wf_term_conv_r : forall l c1 c2 c3 e1 e2 t1 t2 t3,
+    le_subst l c1 c2 s1 s2 c1' c2' ->
+    le_sort l c1' c2' t1' t2' ->
+    le_sort l c1 c2 t1'[/s1/] t2'[/s2/]
+| le_sort_refl : forall l c t,
     (* presuppositions *)
     wf_lang l ->
-    wf_ctxt l c1 c3 ->
-    wf_sort l c1 c3 t1 t3 ->
+    wf_ctx l c ->
+    le_ctx l c c ->
+    wf_sort l c t ->
     (* well-formed input *)
-    wf_term l c1 c2 e1 e2 t1 t2 ->
-    wf_sort l c2 c3 t2 t3 ->
-    wf_term l c1 c3 e1 e2 t1 t3
-| wf_term_conv_l : forall l c1 c2 c3 e2 e3 t1 t2 t3,
+    List.In ({| c |- t }) l ->
+    le_sort l c c t t
+| le_sort_trans : forall l c1 c12 c2 t1 t12 t2,
     (* presuppositions *)
     wf_lang l ->
-    wf_ctxt l c1 c3 ->
-    wf_sort l c1 c3 t1 t3 ->
+    wf_ctx l c1 ->
+    wf_ctx l c2 ->
+    le_ctx l c1 c2 ->
+    wf_sort l c1 t1 ->
+    wf_sort l c2 t2 ->
     (* well-formed input *)
-    wf_term l c2 c3 e2 e3 t2 t3 ->
-    wf_sort l c1 c2 t1 t2 ->
-    wf_term l c1 c3 e2 e3 t1 t3
-with wf_subst {p} : lang p ->
-                    ctxt p -> ctxt p ->
-                    psubst p -> psubst p ->
-                    ctxt p -> ctxt p -> Prop :=
-| wf_subst_nil : forall l c1 c2 c1' c2',
+    le_sort l c1 c12 t1 t12 ->
+    le_sort l c12 c2 t12 t2 ->
+    le_sort l c1 c2 t1 t2
+with wf_term {p} : lang p -> ctx p -> exp p -> exp p -> Prop :=
+| wf_term_by : forall l c e t,
+    (* presuppositions *)
+    wf_lang l ->
+    wf_ctx l c ->
+    wf_sort l c t ->
+    (* well-formed input *)
+    List.In ({| c |- e .: t}) l ->
+    wf_term l c e t
+| wf_term_subst : forall l c s c' e' t',
+    (* presuppositions *)
+    wf_lang l ->
+    wf_ctx l c ->
+    wf_sort l c t'[/s/] ->
+    (* well-formed input *)
+    wf_subst l c s c' ->
+    wf_term l c' e' t' ->
+    wf_term l c e'[/s/] t'[/s/]
+(* terms can be lifted to greater (less precise) types,
+   but not the other way around
+ *)
+| wf_term_conv : forall l c e t c' t',
+    (* presuppositions *)
+    wf_lang l ->
+    wf_ctx l c' ->
+    wf_sort l c' t' ->
+    (* well-formed input *)
+    wf_term l c e t ->
+    le_sort l c c' t t' ->
+    wf_term l c' e t'
+with le_term {p} : lang p ->
+                   ctx p -> ctx p ->
+                   exp p -> exp p ->
+                   exp p -> exp p -> Prop :=
+| le_term_by : forall l c1 c2 e1 e2 t1 t2,
+    (* presuppositions *)
+    wf_lang l ->
+    wf_ctx l c1 ->
+    wf_ctx l c2 ->
+    le_ctx l c1 c2 ->
+    wf_sort l c1 t1 ->
+    wf_sort l c1 t2 ->
+    le_sort l c1 c2 t1 t2 ->
+    wf_term l c1 e1 t1 ->
+    wf_term l c2 e2 t2 ->
+    (* well-formed input *)
+    List.In ({< c1 <# c2|- e1 <# e2 .: t1 <# t2}) l ->
+    le_term l c1 c2 e1 e2 t1 t2
+| le_term_subst : forall l c1 c2 s1 s2 c1' c2' e1' e2' t1' t2',
+    (* presuppositions *)
+    wf_lang l ->
+    wf_ctx l c1 ->
+    wf_ctx l c2 ->
+    le_ctx l c1 c2 ->
+    wf_sort l c1 t1'[/s1/] ->
+    wf_sort l c1 t1'[/s2/] ->
+    le_sort l c1 c2 t1'[/s1/] t1'[/s2/] ->
+    wf_term l c1 e1'[/s1/] t1'[/s1/] ->
+    wf_term l c2 e2'[/s2/] t2'[/s2/] ->
+    (* well-formed input *)
+    le_subst l c1 c2 s1 s2 c1' c2' ->
+    le_term l c1' c2' e1' e2' t1' t2' ->
+    le_term l c1 c2 e1'[/s1/] e2'[/s2/] t1'[/s1/] t2'[/s2/]
+| le_term_refl : forall l c e t,
+    (* presuppositions *)
+    wf_lang l ->
+    wf_ctx l c ->
+    le_ctx l c c ->
+    wf_sort l c t ->
+    le_sort l c c t t ->
+    wf_term l c e t ->
+    (* well-formed input *)
+    List.In ({| c |- e .: t }%rule) l ->
+    le_term l c c e e t t
+| le_term_trans : forall l c1 c12 c2 e1 e12 e2 t1 t12 t2,
+    (* presuppositions *)
+    wf_lang l ->
+    wf_ctx l c1 ->
+    wf_ctx l c2 ->
+    le_ctx l c1 c2 ->
+    wf_sort l c1 t1 ->
+    wf_sort l c1 t2 ->
+    le_sort l c1 c2 t1 t2 ->
+    wf_term l c1 e1 t1 ->
+    wf_term l c2 e2 t2 ->
+    (* well-formed input *)
+    le_term l c1 c12 e1 e12 t1 t12 ->
+    le_term l c12 c2 e12 e2 t12 t2 ->
+    le_term l c1 c2 e1 e2 t1 t2
+(* Conversion:
+
+c1  < c2  |- e1 < e2 : t1  < t2   ||
+/\    /\               /\    /\   ||
+c1' < c2' |- e1 < e2 : t1' < t2'  \/
+*)
+| le_term_conv : forall l c1 c2 e1 e2 t1 t2 c1' c2' t1' t2',
+    (* presuppositions *)
+    wf_lang l ->
+    wf_ctx l c1' ->
+    wf_ctx l c2' ->
+    le_ctx l c1' c2' ->
+    wf_sort l c1' t1' ->
+    wf_sort l c1' t2' ->
+    (* this presupposition is necessary*)
+    le_sort l c1' c2' t1' t2' ->
+    wf_term l c1' e1 t1' ->
+    wf_term l c2' e2 t2' ->
+    (* well-formed input *)
+    le_term l c1 c2 e1 e2 t1 t2 ->
+    le_sort l c1 c1' t1 t1' ->
+    le_sort l c2 c2' t2 t2' ->
+    le_term l c1' c2' e1 e2 t1' t2'
+with wf_subst {p} : lang p -> ctx p -> subst p ->  ctx p -> Prop :=
+| wf_subst_nil : forall l c c',
+    (* presuppositions *)
+    wf_lang l ->
+    wf_ctx l c ->
+    wf_ctx l c' ->
+    (* well-formed input entirely from presuppositions *)
+    wf_subst l c [::] c'
+| wf_subst_sort : forall l c s c' t,
+    (* presuppositions *)
+    wf_lang l ->
+    wf_ctx l c ->
+    wf_ctx l c' ->
+    (* well-formed input *)
+    wf_subst l c s c' ->
+    wf_sort l c t ->
+    wf_subst l c (t::s) c'
+| wf_subst_term : forall l c s c' e t,
+    (* presuppositions *)
+    wf_lang l ->
+    wf_ctx l c ->
+    wf_ctx l (term_var t::c') ->
+    (* well-formed input *)
+    wf_subst l c s c' ->
+    wf_term l c e t[/s/] ->
+    wf_subst l c (e::s) (term_var t::c')
+with le_subst {p} : lang p ->
+                    ctx p -> ctx p ->
+                    subst p -> subst p ->
+                    ctx p -> ctx p -> Prop :=
+| le_subst_nil : forall l c1 c2 c1' c2',
+    (* presuppositions *)
+    wf_lang l ->
+    wf_ctx l c1 ->
+    wf_ctx l c2 ->
+    le_ctx l c1 c2 ->
+    wf_ctx l c1' ->
+    wf_ctx l c2' ->
+    le_ctx l c1' c2' ->
+    wf_subst l c1 [::] c1' ->
+    wf_subst l c2 [::] c2' ->
+    (* well-formed input entirely from presuppositions *)
+    le_subst l c1 c2 [::] [::] c1' c2'
+| le_subst_sort : forall l c1 c2 s1 s2 c1' c2' t1 t2,
+    (* presuppositions *)
+    wf_lang l ->
+    wf_ctx l c1 ->
+    wf_ctx l c2 ->
+    le_ctx l c1 c2 ->
+    wf_ctx l (sort_var::c1') ->
+    wf_ctx l (sort_var::c2') ->
+    le_ctx l (sort_var::c1') (sort_var::c2') ->
+    wf_subst l c1 (t1::s1) (sort_var::c1') -> 
+    wf_subst l c2 (t2::s2) (sort_var::c2') -> 
+    (* well-formed input *)
+    le_subst l c1 c2 s1 s2 c1' c2' ->
+    le_sort l c1 c2 t1 t2 ->
+    le_subst l c1 c2 (t1::s1) (t2::s2) (sort_var::c1') (sort_var::c2')
+| le_subst_term : forall l c1 c2 s1 s2 c1' c2' e1 e2 t1 t2,
+    (* presuppositions *)
+    wf_lang l ->
+    wf_ctx l c1 ->
+    wf_ctx l c2 ->
+    le_ctx l c1 c2 ->
+    wf_ctx l (term_var t1::c1') ->
+    wf_ctx l (term_var t2 :: c2') ->
+    le_ctx l (term_var t1::c1') (term_var t2 :: c2') ->
+    wf_subst l c1 (e1::s1) (term_var t1::c1') -> 
+    wf_subst l c2 (e2::s2) (term_var t2 :: c2') -> 
+    (* well-formed input *)
+    le_subst l c1 c2 s1 s2 c1' c2' ->
+    le_term l c1 c2 e1 e2 t1[/s1/] t2[/s1/] ->
+    le_subst l c1 c2 (e1::s1) (e2::s2) (term_var t1::c1') (term_var t2 :: c2')
+with wf_ctx_var {p} : lang p -> ctx p -> ctx_var p -> Prop :=
+| wf_sort_var : forall l c, 
+    (* presuppositions *)
+    wf_lang l ->
+    wf_ctx l c ->
+    (* well-formed input from presuppositions *)
+    wf_ctx_var l c sort_var
+| wf_term_var : forall l c t, 
+    (* presuppositions *)
+    wf_lang l ->
+    wf_ctx l c ->
+    (* well-formed input *)
+    wf_sort l c t ->
+    wf_ctx_var l c (term_var t)
+with le_ctx_var {p} : lang p -> ctx p -> ctx p -> ctx_var p -> ctx_var p -> Prop :=
+| le_sort_var : forall l c1 c2, 
+    (* presuppositions *)
+    wf_lang l ->
+    wf_ctx l c1 ->
+    wf_ctx l c2 ->
+    le_ctx l c1 c2 ->
+    wf_ctx_var l c1 sort_var ->
+    wf_ctx_var l c2 sort_var ->
+    (* well-formed input from presuppositions *)
+    le_ctx_var l c1 c2 sort_var sort_var
+| le_term_var : forall l c1 c2 t1 t2, 
+    (* presuppositions *)
+    wf_lang l ->
+    wf_ctx l c1 ->
+    wf_ctx l c2 ->
+    le_ctx l c1 c2 ->
+    wf_ctx_var l c1 (term_var t1) ->
+    wf_ctx_var l c2 (term_var t2) ->
+    (* well-formed input *)
+    le_sort l c1 c2 t1 t2 ->
+    le_ctx_var l c1 c2 (term_var t1) (term_var t2)
+with wf_ctx {p} : lang p -> ctx p -> Prop :=
+| wf_ctx_nil : forall l, wf_lang l -> wf_ctx l [::]
+| wf_ctx_cons : forall l c v,
     (* presuppositions *)
     wf_lang l ->
     (* well-formed input *)
-    wf_ctxt l c1 c2 ->
-    wf_ctxt l c1' c2' ->
-    wf_subst l c1 c2 [::] [::] c1' c2'
-| wf_subst_cons_sort : forall l c1 c2 s1 s2 c1' c2' t1 t2,
+    wf_ctx_var l c v ->
+    wf_ctx l (v::c)
+with le_ctx {p} : lang p -> ctx p -> ctx p -> Prop :=
+| le_ctx_nil : forall l, wf_lang l -> le_ctx l [::] [::]
+| le_ctx_cons : forall l c1 c2 v1 v2,
     (* presuppositions *)
     wf_lang l ->
-    wf_ctxt l c1 c2 ->
-    wf_ctxt l (sort_var::c1') (sort_var::c2') ->
+    wf_ctx l (v1::c1) ->
+    wf_ctx l (v2::c2) ->
     (* well-formed input *)
-    wf_subst l c1 c2 s1 s2 c1' c2' ->
-    wf_sort l c1 c2 t1 t2 ->
-    wf_subst l c1 c2 (t1::s1) (t2::s2) (sort_var::c1') (sort_var::c2')
-| wf_subst_cons_term : forall l c1 c2 s1 s2 c1' c2' e1 e2 t1 t2,
-    (* presuppositions *)
-    wf_lang l ->
-    wf_ctxt l c1 c2 ->
-    wf_ctxt l (term_var t1::c1') (term_var t2::c2') ->
-    (* well-formed input *)
-    wf_subst l c1 c2 s1 s2 c1' c2' ->
-    wf_term l c1 c2 e1 e2 t1 t2 ->
-    wf_subst l c1 c2 (e1::s1) (e2::s2) (term_var t1::c1') (term_var t2::c2')
-with wf_ctxt_var {p} : lang p -> ctxt p -> ctxt p -> ctxt_var p -> ctxt_var p -> Prop :=
-| wf_sort_var : forall l c1 c2,
-    (* presuppositions *)
-    wf_lang l ->
-    (* well-formed input *)
-    wf_ctxt l c1 c2 ->
-    wf_ctxt_var l c1 c2 sort_var sort_var
-| wf_term_var : forall l c1 c2 t1 t2,
-    (* presuppositions *)
-    wf_lang l ->
-    (* well-formed input *)
-    wf_sort l c1 c2 t1 t2 ->
-    wf_ctxt_var l c1 c2 (term_var t1) (term_var t2)
-with wf_ctxt {p} : lang p -> ctxt p -> ctxt p -> Prop :=
-| wf_ctxt_nil : forall l, wf_lang l -> wf_ctxt l [::] [::]
-| wf_ctxt_cons : forall l c1 c2 v1 v2,
-    (* presuppositions *)
-    wf_lang l ->
-    wf_ctxt l c1 c2 ->
-    (* well-formed input *)
-    wf_ctxt_var l c1 c2 v1 v2 ->
-    wf_ctxt l (v1::c1) (v2::c2)
+    le_ctx l c1 c2 ->
+    le_ctx_var l c1 c2 v1 v2 ->
+    le_ctx l (v1::c1) (v2::c2)
 with wf_rule {p} : lang p -> rule p -> Prop :=
-| wf_sort_rule : forall l c1 c2 t1 t2,
+| wf_sort_rule : forall l c t,
     (* presuppositions *)
     wf_lang l ->
-    (* well-formed input *)
-    wf_ctxt l c1 c2 ->
-    wf_rule l ({r c1 <# c2 |- t1 <# t2})
-| wf_term_rule : forall l c1 c2 e1 e2 t1 t2,
+    wf_ctx l c ->
+    (* TODO: require t not in thy? *)
+    (* well-formed input from presuppositions *)
+    wf_rule l ({| c |- t})
+| wf_term_rule : forall l c e t,
     (* presuppositions *)
     wf_lang l ->
-    wf_ctxt l c1 c2 ->
-    (* well-formed input *)
-    wf_sort l c1 c2 t1 t2 ->
-    wf_rule l ({r c1 <# c2 |- e1 <# e2 .: t1 <# t2})
-(* TODO: I make common use of this dependent list structure. Codify?*)
+    wf_ctx l c ->
+    wf_sort l c t ->
+    (* TODO: require e not in thy? *)
+    (* well-formed input from presuppositions *)
+    wf_rule l ({| c |- e .: t})
+| le_sort_rule : forall l c1 c2 t1 t2,
+    (* presuppositions *)
+    wf_lang l ->
+    wf_ctx l c1 ->
+    wf_ctx l c2 ->
+    le_ctx l c1 c2 ->
+    wf_sort l c1 t1 ->
+    wf_sort l c2 t2 ->
+    le_sort l c1 c2 t1 t2 ->
+    (* well-formed input from presuppositions *)
+    wf_rule l ({< c1 <# c2 |- t1 <# t2})
+| le_term_rule : forall l c1 c2 e1 e2 t1 t2,
+    (* presuppositions *)
+    wf_lang l ->
+    wf_ctx l c1 ->
+    wf_ctx l c2 ->
+    le_ctx l c1 c2 ->
+    wf_sort l c1 t1 ->
+    wf_sort l c2 t2 ->
+    le_sort l c1 c2 t1 t2 ->
+    wf_term l c1 e1 t1 ->
+    wf_term l c2 e2 t2 ->
+    (* well-formed input from presuppositions *)
+    wf_rule l ({< c1 <# c2 |- e1 <# e2 .: t1 <# t2})
 with wf_lang {p} : lang p -> Prop :=
 | wf_lang_nil : wf_lang [::]
 | wf_lang_cons : forall l r,
-    (* presuppositions *)
-    wf_lang l ->
     (* well-formed input *)
+    wf_lang l ->
     wf_rule l r ->
     wf_lang (r::l).
+
+Section Minimal.
+  (* data type with minimal presuppositions *)
+
 
 (* well-typed sorts, terms are the reflexive case *)
 Definition wf_sort' p l c s : Prop := @wf_sort p l c c s s.
 Definition wf_term' p l c e s : Prop := @wf_term p l c c e e s s.
 Definition wf_subst' p l c s c' : Prop := @wf_subst p l c c s s c' c'.
-Definition wf_ctxt' p l c : Prop := @wf_ctxt p l c c.
+Definition wf_ctx' p l c : Prop := @wf_ctx p l c c.
 
 Create HintDb wf_hints discriminated.
 
 (* well-formed language suppositions *)
-Lemma wf_ctxt_lang  {p} (l : lang p) c1 c2
-      (wfc : wf_ctxt l c1 c2) : wf_lang l.
+Lemma wf_ctx_lang  {p} (l : lang p) c1 c2
+      (wfc : wf_ctx l c1 c2) : wf_lang l.
   case: wfc => //=.
 Qed.
-Hint Immediate wf_ctxt_lang : wf_hints.
-Lemma wf_ctxt_var_lang  {p} (l : lang p) c1 c2 v1 v2
-           (wf : wf_ctxt_var l c1 c2 v1 v2) : wf_lang l.
+Hint Immediate wf_ctx_lang : wf_hints.
+Lemma wf_ctx_var_lang  {p} (l : lang p) c1 c2 v1 v2
+           (wf : wf_ctx_var l c1 c2 v1 v2) : wf_lang l.
   case: wf => //=.
 Qed.
-Hint Immediate wf_ctxt_var_lang : wf_hints.
+Hint Immediate wf_ctx_var_lang : wf_hints.
 Lemma wf_sort_lang  {p} (l : lang p) c1 c2 t1 t2
            (wf : wf_sort l c1 c2 t1 t2) : wf_lang l.
   case: wf => //=.
@@ -503,31 +408,31 @@ Qed.
 Hint Immediate wf_rule_lang : wf_hints.
 
 (* well-formed context suppositions *)
-Lemma wf_sort_ctxt  {p} (l : lang p) c1 c2 t1 t2
-           (wf : wf_sort l c1 c2 t1 t2) : wf_ctxt l c1 c2.
+Lemma wf_sort_ctx  {p} (l : lang p) c1 c2 t1 t2
+           (wf : wf_sort l c1 c2 t1 t2) : wf_ctx l c1 c2.
   case: wf => //=.
 Qed.
-Hint Immediate wf_sort_ctxt : wf_hints.
-Lemma wf_ctxt_var_ctxt  {p} (l : lang p) c1 c2 v1 v2
-           (wf : wf_ctxt_var l c1 c2 v1 v2) : wf_ctxt l c1 c2.
-  case: wf => //= l' c1' c2' t1 t2 _ /wf_sort_ctxt //=.
+Hint Immediate wf_sort_ctx : wf_hints.
+Lemma wf_ctx_var_ctx  {p} (l : lang p) c1 c2 v1 v2
+           (wf : wf_ctx_var l c1 c2 v1 v2) : wf_ctx l c1 c2.
+  case: wf => //= l' c1' c2' t1 t2 _ /wf_sort_ctx //=.
 Qed.
-Hint Immediate wf_ctxt_var_ctxt : wf_hints.
-Lemma wf_term_ctxt  {p} (l : lang p) c1 c2 e1 e2 t1 t2
-           (wf : wf_term l c1 c2 e1 e2 t1 t2) : wf_ctxt l c1 c2.
+Hint Immediate wf_ctx_var_ctx : wf_hints.
+Lemma wf_term_ctx  {p} (l : lang p) c1 c2 e1 e2 t1 t2
+           (wf : wf_term l c1 c2 e1 e2 t1 t2) : wf_ctx l c1 c2.
   case: wf => //=.
 Qed.
-Hint Immediate wf_term_ctxt : wf_hints.
-Lemma wf_subst_ctxt  {p} (l : lang p) c1 c2 s1 s2 c1' c2'
-           (wf : wf_subst l c1 c2 s1 s2 c1' c2') : wf_ctxt l c1 c2.
+Hint Immediate wf_term_ctx : wf_hints.
+Lemma wf_subst_ctx  {p} (l : lang p) c1 c2 s1 s2 c1' c2'
+           (wf : wf_subst l c1 c2 s1 s2 c1' c2') : wf_ctx l c1 c2.
   case: wf => //=.
 Qed.
-Hint Immediate wf_subst_ctxt : wf_hints.
-Lemma wf_subst_ctxt_out  {p} (l : lang p) c1 c2 s1 s2 c1' c2'
-           (wf : wf_subst l c1 c2 s1 s2 c1' c2') : wf_ctxt l c1' c2'.
+Hint Immediate wf_subst_ctx : wf_hints.
+Lemma wf_subst_ctx_out  {p} (l : lang p) c1 c2 s1 s2 c1' c2'
+           (wf : wf_subst l c1 c2 s1 s2 c1' c2') : wf_ctx l c1' c2'.
   case: wf => //=.
 Qed.
-Hint Immediate wf_subst_ctxt_out : wf_hints.
+Hint Immediate wf_subst_ctx_out : wf_hints.
 
 (* well-formed sort presuppositions *)
 Lemma wf_term_sort {p} (l : lang p) c1 c2 e1 e2 t1 t2
@@ -544,21 +449,21 @@ Hint Immediate wf_term_sort : wf_hints.
 (* TODO: should I have another variant w/ the same parameter improvement
    but keeping all of the presuppositions?
    I could call the m wf...intro and wf...elim)*)
-Variant wf_ctxt_ {p} (l : lang p) : ctxt p -> ctxt p -> Prop :=
-| wf_ctxt_nil_ : wf_lang l -> wf_ctxt_ l [::] [::]
-| wf_ctxt_cons_ : forall c1 c2 v1 v2,
-    wf_ctxt_var l c1 c2 v1 v2 ->
-    wf_ctxt_ l (v1::c1) (v2::c2).
-Hint Constructors wf_ctxt_.
+Variant wf_ctx_ {p} (l : lang p) : ctx p -> ctx p -> Prop :=
+| wf_ctx_nil_ : wf_lang l -> wf_ctx_ l [::] [::]
+| wf_ctx_cons_ : forall c1 c2 v1 v2,
+    wf_ctx_var l c1 c2 v1 v2 ->
+    wf_ctx_ l (v1::c1) (v2::c2).
+Hint Constructors wf_ctx_.
 
-Variant wf_ctxt_var_ {p} (l : lang p) (c1 c2 : ctxt p) : ctxt_var p -> ctxt_var p -> Prop :=
-| wf_sort_var_ : wf_ctxt l c1 c2 -> wf_ctxt_var_ l c1 c2 sort_var sort_var
+Variant wf_ctx_var_ {p} (l : lang p) (c1 c2 : ctx p) : ctx_var p -> ctx_var p -> Prop :=
+| wf_sort_var_ : wf_ctx l c1 c2 -> wf_ctx_var_ l c1 c2 sort_var sort_var
 | wf_term_var_ : forall t1 t2,
     wf_sort l c1 c2 t1 t2 ->
-    wf_ctxt_var_ l c1 c2 (term_var t1) (term_var t2).
-Hint Constructors wf_ctxt_var_.
+    wf_ctx_var_ l c1 c2 (term_var t1) (term_var t2).
+Hint Constructors wf_ctx_var_.
 
-Variant wf_sort_ {p} (l : lang p) (c1 c2 : ctxt p) : poly_fix p -> poly_fix p -> Prop :=
+Variant wf_sort_ {p} (l : lang p) (c1 c2 : ctx p) : poly_fix p -> poly_fix p -> Prop :=
 | wf_sort_by_ : forall t1 t2 s1 s2 c1' c2',
     (* TODO: remove this presupposition *)
     wf_sort l c1 c2 t1 t2 ->
@@ -573,7 +478,7 @@ Variant wf_sort_ {p} (l : lang p) (c1 c2 : ctxt p) : poly_fix p -> poly_fix p ->
 Hint Constructors wf_sort_.
 
 
-Variant wf_term_ {p} (l : lang p) (c1 c2 : ctxt p)
+Variant wf_term_ {p} (l : lang p) (c1 c2 : ctx p)
   : poly_fix p -> poly_fix p -> poly_fix p -> poly_fix p -> Prop :=
 | wf_term_by_ : forall e1 e2 t1 t2 s1 s2 c1' c2',
     wf_subst l c1 c2 s1 s2 c1' c2' ->
@@ -601,28 +506,28 @@ Ltac hypothesize :=
 
 Ltac solve_wf_lang :=
   match goal with
-  | [H : wf_ctxt ?l _ _ |- wf_lang ?l] => apply: wf_ctxt_lang; exact H
-  | [H : wf_ctxt_var ?l _ _ _ _ |- wf_lang ?l] => apply: wf_ctxt_var_lang; exact H
+  | [H : wf_ctx ?l _ _ |- wf_lang ?l] => apply: wf_ctx_lang; exact H
+  | [H : wf_ctx_var ?l _ _ _ _ |- wf_lang ?l] => apply: wf_ctx_var_lang; exact H
   | [H : wf_sort ?l _ _ _ _ |- wf_lang ?l] => apply: wf_sort_lang; exact H
   | [H : wf_term ?l _ _ _ _ _ _ |- wf_lang ?l] => apply: wf_term_lang; exact H
   | [H : wf_subst ?l _ _ _ _ _ _ |- wf_lang ?l] => apply: wf_subst_lang; exact H
   | [H : wf_rule ?l _ |- wf_lang ?l] => apply: wf_rule_lang; exact H
   end.
 
-Ltac solve_wf_ctxt :=
+Ltac solve_wf_ctx :=
   match goal with
-  | [H : wf_ctxt_var ?l ?c1 ?c2 _ _ |- wf_ctxt ?l ?c1 ?c2] => apply: wf_ctxt_var_ctxt; exact H
-  | [H : wf_sort ?l ?c1 ?c2 _ _ |- wf_ctxt ?l ?c1 ?c2] => apply: wf_sort_ctxt; exact H
-  | [H : wf_term ?l ?c1 ?c2 _ _ _ _ |- wf_ctxt ?l ?c1 ?c2] => apply: wf_term_ctxt; exact H
-  | [H : wf_subst ?l ?c1 ?c2 _ _ _ _ |- wf_ctxt ?l ?c1 ?c2] => apply: wf_subst_ctxt; exact H
-  | [H : wf_subst ?l _ _ _ _ ?c1 ?c2 |- wf_ctxt ?l ?c1 ?c2] => apply: wf_subst_ctxt_out; exact H
+  | [H : wf_ctx_var ?l ?c1 ?c2 _ _ |- wf_ctx ?l ?c1 ?c2] => apply: wf_ctx_var_ctx; exact H
+  | [H : wf_sort ?l ?c1 ?c2 _ _ |- wf_ctx ?l ?c1 ?c2] => apply: wf_sort_ctx; exact H
+  | [H : wf_term ?l ?c1 ?c2 _ _ _ _ |- wf_ctx ?l ?c1 ?c2] => apply: wf_term_ctx; exact H
+  | [H : wf_subst ?l ?c1 ?c2 _ _ _ _ |- wf_ctx ?l ?c1 ?c2] => apply: wf_subst_ctx; exact H
+  | [H : wf_subst ?l _ _ _ _ ?c1 ?c2 |- wf_ctx ?l ?c1 ?c2] => apply: wf_subst_ctx_out; exact H
   end.
 
 Ltac constr_wf :=
   apply: wf_sort_by
     + apply: wf_sort_trans
-    + apply: wf_ctxt_nil
-    + apply: wf_ctxt_cons
+    + apply: wf_ctx_nil
+    + apply: wf_ctx_cons
     + apply: wf_sort_var
     + apply: wf_term_var
     + apply: wf_term_by
@@ -630,8 +535,8 @@ Ltac constr_wf :=
     + apply: wf_term_conv_l
     + apply: wf_term_conv_r
     (* good variants *)
-    + apply: wf_ctxt_nil_
-    + apply: wf_ctxt_cons_
+    + apply: wf_ctx_nil_
+    + apply: wf_ctx_cons_
     + apply: wf_sort_by_
     + apply: wf_sort_trans_
     + apply: wf_sort_var_
@@ -646,31 +551,31 @@ Ltac solve_wf :=
   by hypothesize;
   constr_wf;
   do [solve_wf_lang
-     | solve_wf_ctxt
+     | solve_wf_ctx
      | eauto].
   
-Lemma wf_ctxt_conv p (l : lang p) c1 c2 : wf_ctxt l c1 c2 <-> wf_ctxt_ l c1 c2.
+Lemma wf_ctx_conv p (l : lang p) c1 c2 : wf_ctx l c1 c2 <-> wf_ctx_ l c1 c2.
 Proof.
   split; case; solve_wf.
 Qed.
-Hint Resolve <- wf_ctxt_conv 0 : wf_hints.
-Coercion ctxt_coerce p (l : lang p) c1 c2 := fst (wf_ctxt_conv l c1 c2).
+Hint Resolve <- wf_ctx_conv 0 : wf_hints.
+Coercion ctx_coerce p (l : lang p) c1 c2 := fst (wf_ctx_conv l c1 c2).
 
-Lemma wf_ctxt_var_conv p (l : lang p) c1 c2 v1 v2
-  : wf_ctxt_var l c1 c2 v1 v2 <-> wf_ctxt_var_ l c1 c2 v1 v2.
+Lemma wf_ctx_var_conv p (l : lang p) c1 c2 v1 v2
+  : wf_ctx_var l c1 c2 v1 v2 <-> wf_ctx_var_ l c1 c2 v1 v2.
 Proof.
   split; case; solve_wf.
 Qed.
-Hint Resolve <- wf_ctxt_var_conv 0 : wf_hints.
-Coercion ctxt_var_coerce p (l : lang p) c1 c2 v1 v2 := fst (wf_ctxt_var_conv l c1 c2 v1 v2).
+Hint Resolve <- wf_ctx_var_conv 0 : wf_hints.
+Coercion ctx_var_coerce p (l : lang p) c1 c2 v1 v2 := fst (wf_ctx_var_conv l c1 c2 v1 v2).
 
-Fixpoint wf_ctxt_to_trans' (n : nat) p (l : lang p) (c1 c2 c3 :ctxt p) {struct n}
-  : n = 2 * size c1 -> wf_ctxt l c1 c2 -> wf_ctxt l c2 c3 -> wf_ctxt l c1 c3
-with wf_ctxt_var_to_trans' (n : nat) p (l : lang p) c1 c2 c3 v1 v2 v3 {struct n}
+Fixpoint wf_ctx_to_trans' (n : nat) p (l : lang p) (c1 c2 c3 :ctx p) {struct n}
+  : n = 2 * size c1 -> wf_ctx l c1 c2 -> wf_ctx l c2 c3 -> wf_ctx l c1 c3
+with wf_ctx_var_to_trans' (n : nat) p (l : lang p) c1 c2 c3 v1 v2 v3 {struct n}
      : n = (2 * size c1).+1 ->
-       wf_ctxt_var l c1 c2 v1 v2 ->
-       wf_ctxt_var l c2 c3 v2 v3 ->
-       wf_ctxt_var l c1 c3 v1 v3.
+       wf_ctx_var l c1 c2 v1 v2 ->
+       wf_ctx_var l c2 c3 v2 v3 ->
+       wf_ctx_var l c1 c3 v1 v3.
 Proof.
   - refine (match n as n' return n' = 2 * size c1 -> _ -> _ -> _ with
               | 0 => _
@@ -687,13 +592,13 @@ Proof.
       inversion wf1.
       rewrite -H2 in wf2;
         inversion wf2;
-      apply wf_ctxt_conv;
+      apply wf_ctx_conv;
       constructor => //=.
       rewrite -H4 in wf2;
         inversion wf2.
-      apply wf_ctxt_conv;
+      apply wf_ctx_conv;
         constructor => //=.
-      apply: (wf_ctxt_var_to_trans' n0) => //=.
+      apply: (wf_ctx_var_to_trans' n0) => //=.
       rewrite -H3 in neq.
       simpl in neq.
       rewrite mulnSr in neq.
@@ -712,35 +617,35 @@ Proof.
       inversion wf1;
       rewrite <- H6 in wf2;
       inversion wf2;
-        apply wf_ctxt_var_conv;
+        apply wf_ctx_var_conv;
         constructor.
-      * apply: (wf_ctxt_to_trans' n0) => //=.        
+      * apply: (wf_ctx_to_trans' n0) => //=.        
         exact H1.
         done.
       * have wfs13 : wf_sort l c1 c3 t1 t3.
         apply: wf_sort_trans.
         done.
-        apply: (wf_ctxt_to_trans' n0) => //=.
-        apply: wf_sort_ctxt; eauto.
-        apply: wf_sort_ctxt; eauto.
+        apply: (wf_ctx_to_trans' n0) => //=.
+        apply: wf_sort_ctx; eauto.
+        apply: wf_sort_ctx; eauto.
         eauto.
         eauto.
         done.
 Qed. 
 
 
-Lemma wf_ctxt_to_trans p (l : lang p) (c1 c2 c3 :ctxt p)
-  : wf_ctxt l c1 c2 -> wf_ctxt l c2 c3 -> wf_ctxt l c1 c3.
+Lemma wf_ctx_to_trans p (l : lang p) (c1 c2 c3 :ctx p)
+  : wf_ctx l c1 c2 -> wf_ctx l c2 c3 -> wf_ctx l c1 c3.
 Proof.
-  apply: wf_ctxt_to_trans' => //=.
+  apply: wf_ctx_to_trans' => //=.
 Qed.
                                                         
-Lemma wf_ctxt_var_to_trans p (l : lang p) c1 c2 c3 v1 v2 v3
-     : wf_ctxt_var l c1 c2 v1 v2 ->
-       wf_ctxt_var l c2 c3 v2 v3 ->
-       wf_ctxt_var l c1 c3 v1 v3.
+Lemma wf_ctx_var_to_trans p (l : lang p) c1 c2 c3 v1 v2 v3
+     : wf_ctx_var l c1 c2 v1 v2 ->
+       wf_ctx_var l c2 c3 v2 v3 ->
+       wf_ctx_var l c1 c3 v1 v3.
 Proof.
-  apply: wf_ctxt_var_to_trans'; eauto.
+  apply: wf_ctx_var_to_trans'; eauto.
 Qed.
 
 
@@ -755,24 +660,34 @@ Proof.
     move => c12 t1' t12 t3' wf1 wf3.
     apply: wf_sort_trans.
     solve_wf.
-    apply: wf_ctxt_to_trans;
-      apply: wf_sort_ctxt; eauto.
+    apply: wf_ctx_to_trans;
+      apply: wf_sort_ctx; eauto.
     eauto.
     eauto.
 Qed.
 Hint Resolve <- wf_sort_conv 0 : wf_hints.
 Coercion sort_coerce p (l : lang p) c1 c2 t1 t2 := fst (wf_sort_conv l c1 c2 t1 t2).
 
-(*TODO: induction principles using wf_sort_, etc *)
+(*TODO: induction principles using wf_sort_, etc
+  should _ be inductives? probably
+ *)
 Lemma wf_sort_monotone p (l : lang p) c1 c2 t1 t2
-  : wf_sort l c1 c2 t1 t2 -> forall r, wf_rule l r -> wf_sort (r::l) c1 c2 t1 t2.
+  : wf_sort l c1 c2 t1 t2 -> forall r, wf_rule l r -> wf_sort (r::l) c1 c2 t1 t2
+with wf_subst_monotone p (l : lang p) c1 c2 s1 s2 c1' c2'
+     : wf_subst l c1 c2 s1 s2 c1' c2' ->
+       forall r, wf_rule l r -> wf_subst (r::l) c1 c2 s1 s2 c1' c2'.
 Proof.
-  elim.
-  - move => l' c1' c2' t1' t2' s1 s2 c1'' c2''.
-    move => wfl wfc wfs IH wfsb lin r wfr.
+  - case /wf_sort_conv.
+    move => t1' t2' s1 s2 c1'' c2''.
+    move => wfs wfsb lin r wfr.
     rewrite wf_sort_conv.
     apply: wf_sort_by_.
+    apply: wf_sort_monotone; done.
+    apply: wf_subst_monotone; try done.
+    eassumption.
+    
     apply: IH; done.
+    
     (*TODO: needs to be mutual with subst monotone? *)
     
 
@@ -800,7 +715,7 @@ Proof.
   - hypothesize.
     apply:wf_term_by; eauto.
     apply: wf_subst_lang; eauto.
-    apply: wf_subst_ctxt; eauto.
+    apply: wf_subst_ctx; eauto.
     move => l' c1' c12 c2' e1' e2' t1' t12 t2'.
     move => wfl wfc wfs wft wfs'.
     apply:wf_term_conv_r_; eauto.
