coq/Exp.v
@@ -1,0 +1,325 @@
+
+Require Import mathcomp.ssreflect.all_ssreflect.
+Set Implicit Arguments.
+Unset Strict Implicit.
+Unset Printing Implicit Defensive.
+Set Bullet Behavior "Strict Subproofs".
+
+Require Vector.
+
+Definition polynomial := seq (Set * nat).
+Print nth.
+
+Definition zterm : Set * nat := (Empty_set , 0).
+
+
+Unset Elimination Schemes.
+Inductive exp (p : polynomial) : Type :=
+  | var : nat -> exp p
+  | con : forall n, fst (nth zterm p n) ->
+                     Vector.t (exp p) (snd (nth zterm p n)) ->
+                     exp p.
+Set Elimination Schemes.
+
+Arguments var {p}.
+Arguments con {p}.
+
+(*Stronger induction principle w/ better subterm knowledge *)
+Fixpoint exp_ind {p}
+         (P : exp p -> Prop)
+         (IHV : forall n, P(var n))
+         (IHC : forall n s v,
+             Vector.fold_right (fun t : exp p => and (P t)) v True ->
+             P (con n s v))
+         (e : exp p) { struct e} : P e :=
+  match e with
+  | var n => IHV n
+  | con n s v =>
+    let fix loop n v :=
+        match v return Vector.fold_right (fun t => and (P t)) v True with
+        | Vector.nil => I
+        | Vector.cons e' n v' => conj (exp_ind IHV IHC e') (loop n v')
+        end in
+    IHC n s v (loop _ v)
+  end.
+
+Notation "[*]" := (Vector.nil _).
+Notation "[* x ]" := (Vector.cons _ _ x (Vector.nil _)).
+Notation "[* x ; .. ; y ]" := (Vector.cons _ x _ .. (Vector.cons _ y _ (Vector.nil _)) ..).
+
+Notation "[ n | s , v ]" := (con n s v).
+Notation "[{ p } n | s , v ]" := (@con p n s v).
+
+
+Section ExpTest.
+  Definition test1 : polynomial := [:: (unit,1) ; (unit,2) ; (nat,0)].
+  
+  Definition tvar (n : nat) : exp test1 :=
+    [{test1} 2 | n, [*]].
+  
+  Definition prod_test : Vector.t nat 1 := [* 3].
+  Definition prod_test2 : Vector.t nat 3 := [* 3; 5; 4].
+  
+  Definition tlam (e : exp test1) : exp test1 :=
+    [{test1} 0 | tt , [* e]].
+  
+  Definition tapp (e1 e2 : exp test1) : exp test1 :=
+    [{test1} 1 | tt, [* e1; e2]].
+  
+  Definition test1ex : exp test1 := tlam (tlam (tapp (tvar 1) (tvar 0))).
+End ExpTest.
+  
+Inductive ctx_var p : Type :=
+| term_var : exp p -> ctx_var p
+| sort_var : ctx_var p.
+
+Arguments term_var {p} e.
+Arguments sort_var {p}.
+
+Definition ctx p := list (ctx_var p).
+
+(* terms form a category over sorts w/ (empty or constant?) Γ *)
+Inductive rule (p : polynomial) : Type :=
+| sort :  ctx p -> exp p -> rule p
+| term :  ctx p -> exp p -> exp p -> rule p
+| sort_le : ctx p -> ctx p -> exp p -> exp p -> rule p
+| term_le : ctx p -> ctx p -> exp p -> exp p -> exp p -> exp p -> rule p.
+
+Bind Scope rule_scope with rule.
+Delimit Scope rule_scope with rule.
+Local Open Scope rule_scope.
+Notation "{< c1 <# c2 |- s1 <# s2 }" := (sort_le c1 c2 s1 s2) (at level 80) : rule_scope.
+Notation "{< c |- s1 <# s2 }" := (sort_le c c s1 s2) (at level 80):rule_scope.
+Notation "{< c |- s }" := (sort_le c c s s) (at level 80):rule_scope.
+Notation "{< c1 <# c2 |- e1 <# e2 .: s1 <# s2 }" :=
+  (term_le c1 c2 e1 e2 s1 s2) (at level 80) : rule_scope.
+Notation "{< c |- e1 <# e2 .: s1 <# s2 }" :=
+  (term_le c c e1 e2 s1 s2) (at level 80) : rule_scope.
+Notation "{< c |- e1 <# e2 .: s }" :=
+  ({< c |- e1 <# e2 .: s <# s}) (at level 80) : rule_scope.
+Notation "{< c |- e .: s }" := 
+  ({< c |- e <# e.: s}) (at level 80) : rule_scope.
+Notation "{| c |- s }" := 
+  (sort c s) (at level 80) : rule_scope.
+Notation "{| c |- e .: s }" := 
+  (term c e s) (at level 80) : rule_scope.
+
+Definition lang p := list (rule p).
+
+Section SynExample.
+  (*EXAMPLE*)
+  (* syntax of single explicit substitutions *)
+  Definition subst_syn : polynomial :=
+    [:: (nat, 0); (* var (deBruijn) *)
+       (unit, 2) (*subst M[N/0] *)
+    ].
+  
+  Definition sub (m n : exp subst_syn) : exp subst_syn :=
+    [{subst_syn} 1 | tt , [* m; n]].
+  
+  Definition svar (n : nat) : exp subst_syn :=
+    [{subst_syn} 0 | n , [*]].
+  
+  (* equational theory of substitutions *)
+  Definition subst_lang : lang subst_syn :=
+    [:: {< [:: sort_var] |- sub (svar 0) (var 0) <# var 0};
+       {<[:: sort_var; sort_var] |- [{subst_syn} 1 | tt, [* var 0; var 1]]};
+       {<[:: sort_var; sort_var; term_var (var 1)] |- [{subst_syn} 1 | tt, [* var 0; var 2]]};
+       {<[:: sort_var; term_var (var 0); sort_var] |-
+        [{subst_syn} 1 | tt, [* var 1; var 2]] .: var 0};
+       {<[:: sort_var; term_var (var 0); sort_var; term_var (var 2)] |-
+        [{subst_syn} 1 | tt, [* var 1; var 3]] .: var 0}
+    ].
+
+  (*TODO: finish axioms
+    (wf_sort_and_cong ([:: sort_var _; sort_var _],
+    Ccon [++ tt | [* Cvar _ 0; Cvar _ 1]]))
+    ++ (wf_sort_and_cong ([:: sort_var _; sort_var _; term_var (Cvar _ 1)],
+    Ccon [++ tt | [* Cvar _ 0; Cvar _ 2]]))
+    ++ (wf_sort_and_cong ([:: sort_var _; term_var (Cvar _ 0); sort_var _],
+    Ccon [++ tt | [* Cvar _ 1; Cvar _ 2]]))
+      ++ (wf_sort_and_cong ([:: sort_var _; term_var (Cvar _ 0); sort_var _; term_var (Cvar _ 2)],
+      Ccon [++ tt | [* Cvar _ 1; Cvar _ 3]])).
+   *)
+End SynExample.
+  
+Definition subst (p : polynomial) := seq (exp p).
+
+Fixpoint var_lookup {p} (c : subst p) (n : nat) : exp p :=
+  match c , n with
+  | [::], _ => var n (*keep the var if no substitution needed*)
+  | e :: _, 0 => e (*use the element if one is found *)
+  | _ :: c', n'.+1 => var_lookup c' n' (*otherwise decrease both and continue *)
+  end.
+
+Fixpoint exp_subst {p} (e : exp p) (s : subst p) : exp p :=
+  match e with
+  | var n => var_lookup s n
+  | con n s' v => con n s' (Vector.map (fun e => exp_subst e s) v)
+  end.
+
+Notation "e [/ s /]" := (exp_subst e s) (at level 7, left associativity).
+
+(*TODO: this is in the library. Why can't I find it? *)
+Lemma sub_0_r : forall n, n - 0 = n.
+Proof.
+  elim; done.
+Qed.  
+
+Lemma lookup_ge : forall p c n, length c <= n -> @var_lookup p c n = var (n - size c).
+Proof.
+  move => p; elim.
+  move => n _;
+  rewrite sub_0_r //=.
+  move => x l IH; elim.
+  rewrite ltn0; done.
+  move => n _.
+  apply: IH.
+Qed.
+
+Lemma lookup_nth : forall p c n, @var_lookup p c n = nth (var (n - size c)) c n.
+Proof.
+  move => p; elim.
+  move => n;
+  rewrite sub_0_r nth_nil //=.
+  move => x l IH; elim;[done|].
+  move => n _;
+  apply: IH.
+Qed.  
+
+(*TODO*)
+(* Well-scoped languages
+   a presupposition of well-formed languages
+   Written as functions that decide the properties
+ *)
+
+Fixpoint ws_exp {p : polynomial} csz (e : exp p) : bool :=
+  match e with
+  | var n => n < csz
+  | con n s v => Vector.fold_right (fun e f => (ws_exp csz e) && f) v true
+  end.
+
+Definition ws_ctx_var {p : polynomial} csz (v : ctx_var p) : bool :=
+  match v with
+  | sort_var => true
+  | term_var ty => ws_exp csz ty
+  end.
+
+Fixpoint ws_ctx {p : polynomial} (c : ctx p) : bool :=
+  match c with
+  | [::] => true
+  | v :: c' => ws_ctx c' && ws_ctx_var (size c) v
+  end.
+
+Fixpoint ws_lang {p : polynomial} (l : lang p) : bool :=
+  match l with
+  |[::] => true
+  | {| c |- s} :: l' => ws_lang l' && ws_exp (size c) s
+  | {| c |- s .: t} :: l' => ws_lang l' && ws_exp (size c) s && ws_exp (size c) t
+  | {< c1 <# c2 |- s1 <# s2} :: l' => ws_lang l' && ws_exp (size c1) s1 && ws_exp (size c2) s2
+  | {< c1 <# c2 |- e1 <# e2 .: s1 <# s2} :: l' =>
+    ws_lang l' && ws_exp (size c1) e1 && ws_exp (size c2) e2
+            && ws_exp (size c1) s1 && ws_exp (size c2) s2
+  end%rule.
+
+(* replaces m variables with terms with n free vars*)
+Definition ws_subst {p} n (s : subst p) m : bool :=
+  (List.fold_right (fun e b => ws_exp n e && b) true s) && (size s == m).
+
+
+Lemma unandb : forall (a b : bool) (C : Prop), (a -> b -> C) <-> (a && b -> C).
+Proof.
+  move => a b C; split.
+  - move => CF ab.
+    apply andb_prop in ab.
+    case: ab.
+    done.
+  - move => CF aa bb.
+    apply CF.
+    rewrite andb_true_intro //=.
+Qed.
+
+Lemma ws_nth : forall p n (s : subst p) m e n',
+    ws_subst n s m -> ws_exp n e -> ws_exp n (nth e s n').
+Proof.
+  move => p n ; elim.
+  - move => m e; elim; [done|].
+    move => n' IH //=.
+  - move => x l IH m e.
+    elim => [| n' _].
+    + rewrite /ws_subst //=.
+      repeat case /andb_prop.
+      done.
+    + rewrite /ws_subst //=.
+      repeat case /andb_prop.
+      move => _ lf wse.
+      case: m wse => //= m.
+      rewrite eqSS => wse.
+      apply: IH.
+      rewrite /ws_subst //=.
+      apply andb_true_intro; split. 
+      done.
+      exact wse.
+Qed.
+
+Lemma ws_empty : forall p n m, @ws_subst p n [::] m = (m == 0).
+Proof.
+  move => p n m.
+  rewrite /ws_subst //=.
+Qed.
+
+Lemma ws_lookup : forall p n (s : subst p) (m n' : nat),
+    ws_subst n s m -> n' < m -> ws_exp n (var_lookup s n').
+Proof.  
+  move => p n.
+  elim.  
+  - move => m;
+    elim;
+    move: ws_empty ->;
+    [ move => /eqP -> //=
+    | move => n' IH //= /eqP => -> //=].
+  - move => e l IH m n'.
+    rewrite /ws_subst => //=.
+    (repeat case /andP) => wse sl sr.
+    elim: n' => [ //= | n' _ n'lt].
+    case: m sr n'lt => //= m.
+    move: eqSS -> => n'lt ngm.
+    apply: (IH m n') => //=.
+    rewrite /ws_subst //=.
+    move: n'lt ->.
+    rewrite Bool.andb_true_r //=.
+Qed.
+
+Ltac ws_simpl :=
+  match goal with
+    (* break up ws_subst *)
+    [ |- is_true (ws_subst _ _ _) -> _] =>
+    rewrite /ws_subst;
+    case /andP
+  end.
+
+
+Theorem subst_preserves_ws
+  : forall {p} e (s : subst p) (c c' : ctx p),
+    ws_exp (size c') e ->
+    ws_subst (size c) s (size c') ->
+    ws_exp (size c) (exp_subst e s).
+Proof.
+  move => p e s c c' wse.
+  move => wss.
+  pose (wss' := wss).
+  move: wss'.
+  ws_simpl.
+  move => elem_ws size_eq.
+  pose size_eq' := size_eq.
+  move: size_eq' wse => /eqP <-.
+  elim: e => //= => n.
+  - apply: ws_lookup => //=;
+    move: size_eq => /eqP -> //=.
+  - move => _.
+    elim => //= x n' v IHA IHB.
+    case /andP => xexp rexp.
+    case: IHB => IHB1 IHB2.
+    apply /andP. split; [auto|].
+    move: IHA -> => //=.
+Qed.
